theory/JITFlat2.thy
@@ -1,7 +1,66 @@
-theory JITFlat
+theory JITFlat2
 
 imports JITPer_aux
 begin
+
+
+type_synonym flat_bpf_prog = "x64_bin \<times> (u64 \<times> nat) list \<times> ((u64\<times>u64) list)"
+
+fun jitflat_bpf :: "(nat \<times> u64 \<times> x64_bin) list \<Rightarrow> flat_bpf_prog \<Rightarrow> flat_bpf_prog" where
+"jitflat_bpf [] st = st"| 
+"jitflat_bpf ((num,off,l_bin0)#xs) (l_bin,l_pc,l_jump) = (
+  let curr_pc = of_nat (length l_bin) in 
+    if l_bin0!0 = (0xE9::u8) then \<comment>\<open> TODO: if the first byte is the opcode of cmp? \<close>
+      jitflat_bpf xs (
+        l_bin@l_bin0,
+        l_pc@[(curr_pc,num)],
+        l_jump@ [(of_nat (length l_pc), of_nat (length l_pc) + off)])
+    else
+      jitflat_bpf xs (l_bin@l_bin0, l_pc@[(curr_pc,num)], l_jump)
+)"
+
+fun find_target_pc_in_l_pc :: "((u64\<times>u64) list) \<Rightarrow> u64 \<Rightarrow> u64 option" where
+"find_target_pc_in_l_pc [] _ = None" |
+"find_target_pc_in_l_pc ((x, y)#xs) pc = (
+  if x = pc then Some y
+  else find_target_pc_in_l_pc xs pc
+)"
+
+definition flat_bpf_one_step :: "u64 \<Rightarrow> nat \<Rightarrow> flat_bpf_prog \<Rightarrow> hybrid_state \<Rightarrow> hybrid_state" where
+"flat_bpf_one_step xpc num lp st = (
+  let (l_bin,l_pc,l_jump) = lp in
+  let (pc, xst) = st in
+    case xst of
+    Stuck \<Rightarrow> (pc, Stuck) |
+    Next xpc_old rs m \<Rightarrow> (
+      if xpc \<noteq> xpc_old then \<comment>\<open> In this case, xpc should be equal to xpc_old \<close>
+        (pc, Stuck)
+      else
+        if l_bin!(unat xpc) = (0xE9::u8) then \<comment>\<open> TODO: if the first byte is the opcode of cmp? \<close>
+          \<comment>\<open> case: BPF JMP \<close>
+          case x64_sem 1 l_bin (Next xpc rs m) of
+          Stuck \<Rightarrow> (pc, Stuck) | \<comment>\<open> if one step error, stop, it should be impossible \<close>
+          Next xpc1 rs1 m1 \<Rightarrow> (
+            if rs1 (CR ZF) = 1 then \<comment>\<open> must JUMP \<close>
+              case find_target_pc_in_l_pc l_jump pc of
+              None \<Rightarrow> (pc, Stuck) |
+              Some npc \<Rightarrow>
+                (npc, (Next (fst (l_pc!(unat npc))) rs1 m1)) \<comment>\<open> go to the target address in the jited x64 binary \<close>
+            else \<comment>\<open> donot JUMP \<close>
+              (pc+1, xst)
+          )
+        else
+          \<comment>\<open> case: NOT BPF JMP \<close>
+          (pc+1, x64_sem num l_bin (Next xpc rs m))
+))"
+
+fun flat_bpf_sem :: "nat \<Rightarrow> flat_bpf_prog \<Rightarrow> hybrid_state \<Rightarrow> hybrid_state" where
+"flat_bpf_sem 0 _ hst = hst" |
+"flat_bpf_sem (Suc n) (l_bin,l_pc,l_jump) (pc, xst) = (
+  let (xpc, num) = l_pc!(unat pc) in
+  let (npc, nxst) = flat_bpf_one_step xpc num (l_bin,l_pc,l_jump) (pc, xst) in
+  flat_bpf_sem n (l_bin,l_pc,l_jump) (npc, nxst)
+)"
 
 type_synonym l_pc = "u64 list"
 
@@ -41,15 +100,12 @@ value "(1::i64) > negative_value_of_i64"
 value "(-1::i64) + (2::i64) > negative_value_of_i64"
 
 
-value "x64_encode (Pjcc Cond_e 3 )"
-value "x64_encode (Pjcc Cond_e (-3) )"
-value "x64_decode 0 [0x48,0x01,0xD8]"
 
 fun jitflat :: "(nat \<times> u64 \<times> x64_bin) list \<Rightarrow> x64_bin \<times> l_pc \<times> l_jump \<Rightarrow> x64_bin \<times> l_pc \<times> l_jump " where
   "jitflat [] last_comp = last_comp"| 
   "jitflat ((num,off,l_bin0)#xs) (fst_comp,snd_comp,trd_comp) = 
         (let curr_pc = of_nat (length fst_comp) in 
-         (if l_bin0!0 = (0x0f::u8) then 
+         (if l_bin0!0 = (0xE9::u8) then 
              (jitflat xs (fst_comp@l_bin0, snd_comp@[curr_pc], trd_comp@ [(of_nat (length snd_comp), of_nat (length snd_comp) + off)]))
           else (jitflat xs (fst_comp@l_bin0, snd_comp@[curr_pc], trd_comp))))"
 
@@ -68,30 +124,9 @@ fun jitflat :: "(nat \<times> i64 \<times> x64_bin) list \<Rightarrow> x64_bin \
 definition init_second_layer::"x64_bin \<times> l_pc \<times> l_jump" where
 "init_second_layer \<equiv> ([],[],[])"
 
-definition getIndex ::"u64 \<Rightarrow> l_pc \<Rightarrow> nat" where
-  "getIndex pc snd_comp \<equiv> SOME place. snd_comp!place = pc"
+value "jitflat [(1, 1, [0x48,0x01,0xD8]),(1, 2, [0xE9, 0x00, 0x00, 0x00, 0x00]), (1, 1, [0x48,0x01,0xD8]), (1, 1, [0x48,0x01,0xD8])] init_second_layer"
 
-definition getPair ::"nat \<Rightarrow> l_jump \<Rightarrow> (location\<times>target_pc)" where
-  "getPair idx thrd_comp \<equiv> SOME pair. pair \<in> set thrd_comp \<and> fst pair = of_nat idx"
-
-fun x64_sem2::"nat \<Rightarrow> x64_bin \<times> l_pc \<times> l_jump \<Rightarrow> hybrid_state \<Rightarrow> hybrid_state" where
- "x64_sem2 0 _ st = st" |
- "x64_sem2 (Suc n) (lt,snd_comp,thrd_comp) (pc,xst) = 
-   (let xst' = (if lt!(unat pc) = 0x0f then 
-                    case xst of Stuck \<Rightarrow> Stuck |
-                                Next xpc xrs xm \<Rightarrow>
-                                    let place = getIndex pc snd_comp;
-                                        pair = getPair place thrd_comp;
-                                        target_idx = snd pair;
-                                        target_place = snd_comp !(unat target_idx) in
-                                    Next target_place xrs xm 
-                else x64_sem 1 lt xst) in
-   let off = (case xst' of Stuck \<Rightarrow> pc |
-                           Next pc' rs' m' \<Rightarrow> pc') in
-   x64_sem2 n (lt,snd_comp,thrd_comp) (off,xst'))"
-
-
-
+value "jitflat [(1, 2, [0xE9, 0x00, 0x00, 0x00, 0x00]), (1, 1, [0xc3]), (1, 1, [0x48,0x01,0xD8]), (1, 1, [0x48,0x01,0xD8]),(1, -3, [0xE9, 0x00, 0x00, 0x00, 0x00])] init_second_layer"
 
 value "[0xE9, 0x00, 0x00, 0x00, 0x00]::u8 list "
 
@@ -136,34 +171,20 @@ fun jitfix :: "l_jump \<Rightarrow> x64_bin \<Rightarrow> l_pc \<Rightarrow> x64
   "jitfix [] l _  = l" |
   "jitfix (x#xs) l pcs = (let fix_begin_addr = pcs!(unat (fst x)); 
                               target_begin_addr = pcs!(unat (snd x));
-                              offset = (scast (target_begin_addr)::i32) - (scast(fix_begin_addr+6)::i32);
+                              offset = (scast (target_begin_addr)::i32) - (scast(fix_begin_addr+5)::i32);
                               u8_list = u8_list_of_i32 offset;
-                              l' = x64_bin_update l (unat (fix_begin_addr+2)) u8_list in 
+                              l' = x64_bin_update l (unat (fix_begin_addr+1)) u8_list in 
                           jitfix xs l' pcs)"
 
-value "jitflat [(1, 1, [0x48,0x01,0xD8]),(1, 2, [0x0f, 0x84, 0x00, 0x00, 0x00, 0x00]), (1, 1, [0x48,0x01,0xD8]), (1, 1, [0x48,0x01,0xD8])] init_second_layer"
-
-value "jitflat [(1, 2, [0x0f, 0x84, 0x00, 0x00, 0x00, 0x00]), (1, 1, [0xc3]), (1, 1, [0x48,0x01,0xD8]), (1, 1, [0x48,0x01,0xD8]),(1, -3, [0x0f, 0x84, 0x00, 0x00, 0x00, 0x00])] init_second_layer"
-
 value "jitfix [(1::64 word, 3::64 word)] 
-  [72::8 word, 1::8 word, 216::8 word, 15::8 word, 132::8 word, 0::8 word, 0::8 word, 0::8 word, 0::8 word, 72::8 word, 1::8 word, 216::8 word, 72::8 word, 1::8 word, 216::8 word] 
-  [0::64 word, 3::64 word, 9::64 word, 12::64 word]"
-
-value "jitfix [(0::64 word, 2::64 word), (4::64 word, 1::64 word)] 
-  [15::8 word, 132::8 word, 0::8 word, 0::8 word, 0::8 word, 0::8 word, 195::8 word, 72::8 word, 1::8 word, 216::8 word, 72::8 word, 1::8 word, 216::8 word, 15::8 word, 132::8 word, 0::8 word, 0::8 word, 0::8 word, 0::8 word] 
-  [0::64 word, 6::64 word, 7::64 word, 10::64 word, 13::64 word]"
-(*value "jitfix [(1::64 word, 3::64 word)]
   [72::8 word, 1::8 word, 216::8 word, 233::8 word, 0::8 word, 0::8 word, 0::8 word, 0::8 word, 72::8 word, 1::8 word, 216::8 word, 72::8 word, 1::8 word, 216::8 word]
   [0::64 word, 3::64 word, 8::64 word, 11::64 word]"
 
 value "jitfix [(0::64 word, 2::64 word), (4::64 word, 1::64 word)]
 [233::8 word, 0::8 word, 0::8 word, 0::8 word, 0::8 word, 195::8 word, 72::8 word, 1::8 word, 216::8 word, 72::8 word, 1::8 word, 216::8 word, 233::8 word, 0::8 word, 0::8 word, 0::8 word, 0::8 word]
-[0::64 word, 5::64 word, 6::64 word, 9::64 word, 12::64 word]  "*)
+[0::64 word, 5::64 word, 6::64 word, 9::64 word, 12::64 word]  "
 
 
-
-
-(*
 fun x64_sem2::"nat \<Rightarrow> x64_bin \<Rightarrow> hybrid_state \<Rightarrow> hybrid_state" where
  "x64_sem2 0 _ st = st" |
  "x64_sem2 (Suc n) lt (pc,xst) = 
@@ -171,18 +192,8 @@ fun x64_sem2::"nat \<Rightarrow> x64_bin \<Rightarrow> hybrid_state \<Rightarrow
    off = (case xst' of Stuck \<Rightarrow> pc |
                 Next pc' rs' m' \<Rightarrow> pc') in
     x64_sem2 n lt (off,xst'))"
-*)
 
-lemma refinement_relation_of_two_layers:
-  "snd st = Next pc rs m \<Longrightarrow>
-  x64_sem1 n x64_prog st = st1 \<Longrightarrow>
-  snd st1 = Next pc' rs' m' \<Longrightarrow>
-  (l_bin0, pc_info, jump_info) = jitflat x64_prog init_second_layer \<Longrightarrow>
-  jitfix jump_info l_bin0 pc_info = x64_prog2 \<Longrightarrow>
-  x64_sem2 n x64_prog2 st = st2 \<Longrightarrow>
-  st1 = st2"
-  sorry
-                   
+
 (*
 
 fun x64_sem2::"nat \<Rightarrow> x64_bin \<Rightarrow> hybrid_state \<Rightarrow> hybrid_state" where
@@ -214,6 +225,7 @@ fun jitfix :: "l_jump \<Rightarrow> x64_bin \<Rightarrow> l_pc \<Rightarrow> x64
                               l' = x64_bin_update l (unat (place_end-3)) u8_list in 
                           jitfix xs l' pcs)"
 *)
+value "x64_encode (Pjmp 0x2)"
 
 (*
 fun jitflat1 :: "(nat \<times> u64 \<times> x64_bin) list \<Rightarrow> x64_bin" where
@@ -256,8 +268,20 @@ definition jitflat3 :: "(nat \<times> u64 \<times> x64_bin) list \<Rightarrow> (
     then Some (curr_jump_list !(unat i)) else init_l_jump i))"
 *)
 
+value "x64_encode (Pjmp ((-1)::i32))"
 
-                              
+
+
+lemma refinement_relation_of_two_layers:
+  "snd st = Next pc rs m \<Longrightarrow>
+  x64_sem1 n x64_prog st = st1 \<Longrightarrow>
+  snd st1 = Next pc' rs' m' \<Longrightarrow>
+  (l_bin0, pc_info, jump_info) = jitflat x64_prog init_second_layer \<Longrightarrow>
+  jitfix jump_info l_bin0 pc_info = x64_prog2 \<Longrightarrow>
+  x64_sem2 n x64_prog2 st = st2 \<Longrightarrow>
+  st1 = st2"
+  sorry
+                                                 
 
 
 end
