theory/JITPer.thy
@@ -20,408 +20,15 @@ imports
 
 begin
 
-(*
-lemma demo1: 
+
+lemma one_step_equiv_proof: 
   assumes a0:"s' = sbpf_step prog s" and
   a1:"s = (SBPF_OK pc rs m)" and
   a2:"s' = (SBPF_OK pc' rs' m')" and
   a3:"xst = (Next xpc xrs xm)" and
   a4:"match_state s (pc,xst)" and
   a5:"jitper prog = Some x64_prog" and                      
-  a6:"prog \<noteq> [] \<and> unat pc < length prog \<and> unat pc \<ge> 0" and
-  a7:"xpc = 0"
-shows "\<exists> xst'. let l = (x64_prog!(unat pc)) in x64_sem (fst l) (snd (snd l)) xst = xst' \<and> 
-  match_state s' (pc',xst')"
-(* \<and> snd xst' = unat (pc+1)*)
-proof-
-  let "?bpf_ins" = "prog!(unat pc)"
-  have b0:"length prog \<noteq> 0" using a6 by blast
-  have b1:"(\<exists> src dst. ?bpf_ins = BPF_ALU64 BPF_ADD dst (SOReg src) \<or> ?bpf_ins = BPF_ALU64 BPF_MUL dst (SOReg src))
-  \<or> (\<exists> src dst x cond. ?bpf_ins = BPF_JUMP cond dst (SOReg src) x)" using a0 a1 a2 a6 b0 aux1 by fast
-  obtain src dst x cond where b2:"?bpf_ins = BPF_ALU64 BPF_ADD dst (SOReg src) \<or> ?bpf_ins = BPF_ALU64 BPF_MUL dst (SOReg src) \<or> ?bpf_ins = BPF_JUMP cond dst (SOReg src) x" using b1 by auto
-  show ?thesis
-  proof (cases "?bpf_ins = BPF_ALU64 BPF_ADD dst (SOReg src)")
-    case True
-    let "?l_bin"= "snd (snd (the (per_jit_ins ?bpf_ins)))"
-    have c0:"?l_bin = snd (snd (the (per_jit_add_reg64_1 dst src)))" using b2 True by fastforce
-    have c1:"?l_bin = x64_encode (Paddq_rr (bpf_to_x64_reg dst) (bpf_to_x64_reg src))" using per_jit_add_reg64_1_def c0 by fastforce
-    have c2:"l = ?l_bin" using a6 c0 a5 aux5 by metis
-    let "?st" = "x64_sem num ?l_bin xst"
-    have "x64_prog!(unat pc) = the (per_jit_ins ?bpf_ins)" using aux5 a5 a6 by blast
-    then have "x64_prog!(unat pc) = the (per_jit_add_reg64_1 dst src)" using b2 True by simp
-    then have c3_1:"num = 1" using per_jit_add_reg64_1_def by simp
-    moreover have "list_in_list ?l_bin 0 ?l_bin" using  list_in_list_prop by simp
-    hence "\<exists> xins2. x64_decode 0 ?l_bin = Some (length ?l_bin, xins2) " 
-      using x64_encode_decode_consistency a3 a7 c1 list_in_list_prop c3_1 by blast
-    then obtain xins2 where c3:"x64_decode 0 ?l_bin = Some (length ?l_bin, xins2)" by auto
-    have c4:"?st = exec_instr xins2 (of_nat (length ?l_bin)) xpc xrs xm" using c3 True a3 a7
-      apply(cases xst,simp_all) apply(cases "prog ! unat pc",simp_all) by (simp add: calculation)
-    have c5:"xins2 = Paddq_rr (bpf_to_x64_reg dst) (bpf_to_x64_reg src)" using Pair_inject c4 c3 c1 option.inject x64_encode_decode_consistency list_in_list_prop by metis
-    have c6:"\<exists> xrs' xpc' xm'. ?st = Next xpc' xrs' xm'" using exec_instr_def spec c5 c4 by auto
-    obtain xrs' xpc' xm' where c7:"?st = Next xpc' xrs' xm'" using c6 by auto
-    have "match_state s' (pc',?st)" using addq_subgoal_rr_generic a0 a1 a2 c7 a4 a3 per_jit_add_reg64_1_def b2 c4 c3 True by fastforce
-    then show ?thesis using True b2 c2 by force                                        
-  next
-    case False
-    have c0_0:"?bpf_ins = BPF_ALU64 BPF_MUL dst (SOReg src) \<or> (?bpf_ins = BPF_JUMP cond dst (SOReg src) x)" using False b2 by blast
-    thus ?thesis
-  
-  proof(cases "(?bpf_ins = BPF_JUMP cond dst (SOReg src) x)")
-    case False
-    have c0_1:"?bpf_ins = BPF_ALU64 BPF_MUL dst (SOReg src)" using False c0_0 by simp
-    let "?l_bin"= "snd (snd (the (per_jit_ins ?bpf_ins)))"
-    have c0:"?l_bin = snd (snd (the (per_jit_mul_reg64 dst src)))" using b2 c0_0 False by fastforce
-    let "?result" = "per_jit_mul_reg64 dst src"
-    have c2_0:"(bpf_to_x64_reg dst) = RDX \<or> (bpf_to_x64_reg dst) = RAX \<or> (bpf_to_x64_reg dst) \<notin> {RAX, RDX}" by blast
-    
- thus ?thesis
- proof(cases "(bpf_to_x64_reg dst) = RDX")
-  case True
-    have c2:"(bpf_to_x64_reg dst) = RDX " using True by blast
-    have c1:"?l_bin = (x64_encode (Pmovq_rr R11 (bpf_to_x64_reg src))@(x64_encode (Ppushl_r RAX)) @ (x64_encode (Pmovq_rr RAX RDX)) 
-                  @ (x64_encode (Pmulq_r R11))@(x64_encode (Pmovq_rr RDX RAX))@(x64_encode (Ppopl RAX)))" 
-      using c0 per_jit_mul_reg64_def c2 by auto
-
-
-    let "?l_bin1" = "x64_encode (Pmovq_rr R11 (bpf_to_x64_reg src))"
-    let "?l_bin2" = "x64_encode (Ppushl_r RAX)"
-    let "?l_bin3" = "x64_encode (Pmovq_rr RAX RDX)"
-    let "?l_bin4" = "x64_encode (Pmulq_r R11)"
-    let "?l_bin5" = "x64_encode (Pmovq_rr RDX RAX)"
-    let "?l_bin6" = "x64_encode (Ppopl RAX)"
-    have d1:"list_in_list (?l_bin1@?l_bin2@?l_bin3@?l_bin4@?l_bin5@?l_bin6) (0::nat) ?l_bin " using c1 list_in_list_prop c1 by metis
-    have d2:"list_in_list ?l_bin 0 ?l_bin = 
-      (list_in_list ?l_bin1 0 ?l_bin \<and> list_in_list ?l_bin2 (0 + length ?l_bin1) ?l_bin \<and> 
-       list_in_list ?l_bin3 (0 + length ?l_bin1+length ?l_bin2) ?l_bin \<and> 
-       list_in_list ?l_bin4 (0 + length ?l_bin1+length ?l_bin2+length ?l_bin3) ?l_bin \<and>
-       list_in_list ?l_bin5 (0 + length ?l_bin1+length ?l_bin2+length ?l_bin3+length ?l_bin4) ?l_bin \<and> 
-       list_in_list ?l_bin6 (0 + length ?l_bin1+length ?l_bin2+length ?l_bin3+length ?l_bin4+length ?l_bin5) ?l_bin)" 
-    using list_in_list_concat d1 c1 list_in_list_prop by (smt (verit, ccfv_SIG))
-
-  have d0:"list_in_list ?l_bin1 0 ?l_bin" using c1 by simp
-  have "\<exists> sz1 xins1. x64_decode 0 ?l_bin = Some (sz1,xins1)" using d0 x64_encode_decode_consistency by blast
-  then obtain sz1 xins1 where d3_0:"x64_decode 0 ?l_bin = Some (sz1,xins1)" by auto
-  hence d0_1:"(sz1,xins1) = (3, Pmovq_rr R11 (bpf_to_x64_reg src))" using d0 x64_encode_decode_consistency by fastforce
-  have "\<exists> xpc1 xrs1 m1. exec_instr xins1 (of_nat sz1) xpc xrs xm = Next xpc1 xrs1 m1" 
-    using d0_1 exec_instr_def by(cases xins1,simp_all)
-  then obtain xpc1 xrs1 m1 where b3:"exec_instr xins1 (of_nat sz1) xpc xrs xm = Next xpc1 xrs1 m1" by blast
-  have f0:"3 = length ?l_bin1" using d0_1 by simp
-
-  have d3:"list_in_list ?l_bin2 (0 + length ?l_bin1) ?l_bin" using d1 d2 c1 by argo
-  have "\<exists> sz2 xins2. x64_decode (0 + length ?l_bin1) ?l_bin = Some (sz2,xins2)" using  d0 c1 x64_encode_decode_consistency 
-    using d3 by blast
-  then obtain sz2 xins2 where d4_0:"x64_decode (0 + length ?l_bin1) ?l_bin = Some (sz2,xins2)" by auto
-  hence d4_1:"(sz2,xins2) =(length ?l_bin2,Ppushl_r RAX)" using x64_encode_decode_consistency c1 d0 option.sel d3 by metis
-  hence d4_2:"sz2 = 1 " apply(cases xins2,simp_all)using bitfield_insert_u8_def Let_def construct_rex_to_u8_def by simp
-  have f1:"1 = length ?l_bin2" using d4_2 d4_1 by blast
-  let "?len" = "length (let rex = construct_rex_to_u8 False False False False; op = bitfield_insert_u8 0 3 80 0 in if rex = 64 then [op] else [rex, op])" 
-  have fn:"?len = 1" by(unfold Let_def construct_rex_to_u8_def bitfield_insert_u8_def,simp_all)
-  have "\<exists> st2. exec_instr xins2 (of_nat sz2) xpc1 xrs1 m1 = st2" 
-    using d4_1 d4_2 apply(unfold exec_instr_def) 
-    by(cases xins2,simp_all)
-  then obtain st2 where d4_3:"exec_instr xins2 (of_nat sz2) xpc1 xrs1 m1 = st2" by auto
-  hence "\<exists> xpc2 xrs2 m2. Next xpc2 xrs2 m2 = st2"
-    apply(unfold exec_instr_def) 
-    apply(cases xins2,simp_all) using d4_1 d4_2 d4_3 fn
-         apply(unfold exec_push_def Let_def,simp_all)
-    apply(cases "storev M64 m1 (Vptr ?len (xrs1 (IR SP) - u64_of_memory_chunk M64)) (Vlong (xrs1 (IR RAX)))",simp_all)
-    subgoal for x3 
-      apply(unfold storev_def,simp_all)
-      by (meson option.simps(3))
-    subgoal for x3 a 
-      apply(unfold storev_def sp_block_def,simp_all)
-      by blast
-    done
-  then obtain xpc2 xrs2 m2 where b4:"Next xpc2 xrs2 m2 = exec_instr xins2 (of_nat sz2) xpc1 xrs1 m1" using d4_3 by auto
-
-  have d5:"list_in_list ?l_bin3 (0 + length ?l_bin1+length ?l_bin2) ?l_bin" using d1 c1 d2 by metis
-  hence "\<exists> sz3 xins3. x64_decode (0 + length ?l_bin1+length ?l_bin2) ?l_bin = Some (sz3,xins3)" using c1 x64_encode_decode_consistency by blast
-  then obtain sz3 xins3 where d5_1:"x64_decode (0 + length ?l_bin1+length ?l_bin2) ?l_bin = Some (sz3,xins3)" by auto
-  have d6:"(sz3,xins3) = (length ?l_bin3, Pmovq_rr RAX RDX)" using x64_encode_decode_consistency c1 d3 option.sel d0 d5 d5_1 by metis
-  hence d7:"sz3 = 3" by auto
-  have f2:"length ?l_bin3 = 3" using d6 d7 by simp
-  have "\<exists> xpc3 xrs3 m3. exec_instr xins3 (of_nat sz3) xpc2 xrs2 m2 = Next xpc3 xrs3 m3" 
-    using d6 d7 apply(unfold exec_instr_def) 
-    by(cases xins3,simp_all)  
-  then obtain xpc3 xrs3 m3 where b5:"exec_instr xins3 (of_nat sz3) xpc2 xrs2 m2 = Next xpc3 xrs3 m3" by auto
-
-
-  have d8:"list_in_list ?l_bin4 (0 + length ?l_bin1+length ?l_bin2+length ?l_bin3) ?l_bin" using d1 d2 c1 by metis
-  hence "\<exists> sz4 xins4. x64_decode (0 + length ?l_bin1+length ?l_bin2+length ?l_bin3) ?l_bin = Some (sz4,xins4)" 
-    using c1 x64_encode_decode_consistency by blast
-  then obtain sz4 xins4 where d8_1:"x64_decode (0 + length ?l_bin1+length ?l_bin2+length ?l_bin3) ?l_bin = Some (sz4,xins4)" by auto
-  have d9:"(sz4,xins4) = (length ?l_bin4, Pmulq_r R11)" using x64_encode_decode_consistency c1 d3 option.sel d0 d5 d8 d8_1 by metis
-  hence d10:"sz4 = 3" by auto
-  have f3:"length ?l_bin5 = 3" using d10 d8_1 by simp
-  have "\<exists> xpc4 xrs4 m4. exec_instr xins4 (of_nat sz4) xpc3 xrs3 m3 = Next xpc4 xrs4 m4" 
-    using d9 d10 apply(unfold exec_instr_def)
-    by(cases xins4,simp_all)  
-  then obtain xpc4 xrs4 m4 where b6:"exec_instr xins4 (of_nat sz4) xpc3 xrs3 m3 = Next xpc4 xrs4 m4" by auto
-
-
-  have d11:"list_in_list ?l_bin5 (0 + length ?l_bin1+length ?l_bin2+length ?l_bin3+length ?l_bin4) ?l_bin" using d1 d2 c1 by metis
-  hence "\<exists> sz5 xins5. x64_decode (0 + length ?l_bin1+length ?l_bin2+length ?l_bin3+length ?l_bin4) ?l_bin = Some (sz5,xins5)" 
-    using c1 x64_encode_decode_consistency by blast
-  then obtain sz5 xins5 where d11_1:"x64_decode (0 + length ?l_bin1+length ?l_bin2+length ?l_bin3+length ?l_bin4) ?l_bin = Some (sz5,xins5)" by auto
-  have d12:"(sz5,xins5) = (length ?l_bin5, Pmovq_rr RDX RAX)" using x64_encode_decode_consistency c1 d3 option.sel d0 d5 d8 d9 d11 d11_1 by metis
-  hence d13:"sz5 = 3" by auto
-  have f4:"length ?l_bin5 = 3" using d13 d11_1 by simp
-  have "\<exists> xpc5 xrs5 m5. exec_instr xins5 (of_nat sz5) xpc4 xrs4 m4 = Next xpc5 xrs5 m5"
-    using d12 d13 apply(unfold exec_instr_def)
-    by(cases xins5,simp_all)  
-  then obtain xpc5 xrs5 m5 where b7:"exec_instr xins5 (of_nat sz5) xpc4 xrs4 m4 = Next xpc5 xrs5 m5" by auto
-
- 
-  have d14:"list_in_list ?l_bin6 (0 + length ?l_bin1+length ?l_bin2+length ?l_bin3+length ?l_bin4+length ?l_bin5) ?l_bin" using d1 d2 c1 by metis
-  hence "\<exists> sz6 xins6. x64_decode (0 + length ?l_bin1+length ?l_bin2+length ?l_bin3+length ?l_bin4+length ?l_bin5) ?l_bin = Some (sz6,xins6)" 
-    using c1 x64_encode_decode_consistency by blast
-  then obtain sz6 xins6 where d14_1:"x64_decode (0 + length ?l_bin1+length ?l_bin2+length ?l_bin3+length ?l_bin4+length ?l_bin5) ?l_bin = Some (sz6,xins6)" by auto
-  have d15:"(sz6,xins6) = (length ?l_bin6, Ppopl RAX)" using x64_encode_decode_consistency c1 d3 option.sel d0 d5 d8 d9 d11 d14 d14_1 by metis
-  hence d16:"sz6 = 1" apply(cases xins6,simp_all)using bitfield_insert_u8_def Let_def construct_rex_to_u8_def by simp
-  have f5:"length ?l_bin6 = 1" using d16 d14_1 by (metis d15 prod.inject)
-  have "\<exists> st6. exec_instr xins6 (of_nat sz6) xpc5 xrs5 m5 = st6"
-    using d15 d16 by(cases xins6,simp_all) 
-  then obtain st6 where b8_1:"exec_instr xins6 (of_nat sz6) xpc5 xrs5 m5 = st6" by auto
-  (*hence "\<exists> xpc6 xrs6 m6. st6 = Next xpc6 xrs6 m6"*)
-  
-  let "?xins" = "[(sz1,xins1)]@[(sz2,xins2)]@[(sz3,xins3)]@[(sz4,xins4)]@[(sz5,xins5)]@[(sz6,xins6)]"
-  have c13:"?xins = [(3,Pmovq_rr R11 (bpf_to_x64_reg src)), (1,Ppushl_r RAX), (3,Pmovq_rr RAX RDX), (3,Pmulq_r R11), (3,Pmovq_rr RDX RAX), (1,Ppopl RAX)]"
-    using d0 d0_1 d4_1 d4_2 d6 d7 d9 d10 d12 d13 d16 d15 by auto
-  have c14_1:"exec_instr (snd(?xins!0)) (of_nat(fst(?xins!0))) xpc xrs xm = Next xpc1 xrs1 m1\<and>
-    exec_instr (snd(?xins!1)) (of_nat(fst(?xins!1))) xpc1 xrs1 m1 = Next xpc2 xrs2 m2 \<and>
-    exec_instr (snd(?xins!2)) (of_nat(fst(?xins!2))) xpc2 xrs2 m2 = Next xpc3 xrs3 m3 \<and>
-    exec_instr (snd(?xins!3)) (of_nat(fst(?xins!3))) xpc3 xrs3 m3 = Next xpc4 xrs4 m4 \<and>
-    exec_instr (snd(?xins!4)) (of_nat(fst(?xins!4))) xpc4 xrs4 m4 = Next xpc5 xrs5 m5 \<and> 
-    exec_instr (snd(?xins!5)) (of_nat(fst(?xins!5))) xpc5 xrs5 m5 = st6 " 
-    using b3 b4 b5 b6 b7 b8_1 by simp
-    
-  have b8_2:"st6\<noteq> Stuck" using mulq_subgoal_rr_aux4 c13 c14_1 by fast
-  hence "\<exists> xpc6 xrs6 m6. st6 = Next xpc6 xrs6 m6 "by (meson outcome.exhaust)
-  then obtain xpc6 xrs6 m6 where b8:"Next xpc6 xrs6 m6 = exec_instr xins6 (of_nat sz6) xpc5 xrs5 m5" using b8_1 by auto
-
-  have c14:"exec_instr (snd(?xins!0)) (of_nat(fst(?xins!0))) xpc xrs xm = Next xpc1 xrs1 m1\<and>
-    exec_instr (snd(?xins!1)) (of_nat(fst(?xins!1))) xpc1 xrs1 m1 = Next xpc2 xrs2 m2 \<and>
-    exec_instr (snd(?xins!2)) (of_nat(fst(?xins!2))) xpc2 xrs2 m2 = Next xpc3 xrs3 m3 \<and>
-    exec_instr (snd(?xins!3)) (of_nat(fst(?xins!3))) xpc3 xrs3 m3 = Next xpc4 xrs4 m4 \<and>
-    exec_instr (snd(?xins!4)) (of_nat(fst(?xins!4))) xpc4 xrs4 m4 = Next xpc5 xrs5 m5 \<and> 
-    exec_instr (snd(?xins!5)) (of_nat(fst(?xins!5))) xpc5 xrs5 m5 = Next xpc6 xrs6 m6 " 
-    using c14_1 b8 by simp
-    
-  
-  let "?st'" = "x64_sem num ?l_bin xst" 
-  have c16:"l = ?l_bin" using a6 c0 a5 aux5 by metis
-  have "x64_prog!(unat pc) = the (per_jit_ins ?bpf_ins)" using aux5 a5 a6 by blast
-  then have c5:"x64_prog!(unat pc) = the (per_jit_mul_reg64 dst src)" using b2 c0_0 False by simp
-  have c17:"num = length ?xins" using per_jit_mul_reg64_def c2
-      apply(cases "(bpf_to_x64_reg dst)",simp_all) using c5 by force
-   have c15:"num = (Suc(Suc(Suc(Suc(Suc(Suc 0))))))" using c17 by simp
-  (*let "?st'" = "x64_sem (Suc(Suc(Suc(Suc(Suc(Suc 0)))))) ?l_bin xst" *)
-   (*have cn:"?st' = Next xpc6 xrs6 m6" using c15 b3 b4 b5 b6 b7 b8  d3_0 d4_0 d5_1 d8_1 d11_1 d14_1 sorry*)
-   have c3_1:"x64_decode (unat xpc) ?l_bin \<noteq> None" using a7 using d3_0 by simp
-   hence c3_2:"?st' = (case x64_decode (unat xpc) ?l_bin of
-                  None \<Rightarrow> Stuck |
-                 Some (sz, ins) \<Rightarrow>
-              x64_sem (Suc(Suc(Suc(Suc(Suc 0))))) ?l_bin (exec_instr ins (of_nat sz) xpc xrs xm))" 
-      using a3 c0_1 c15 c0 d3_0 apply(cases xst,simp_all) 
-      apply(cases "prog ! unat pc",simp_all)
-      subgoal for x91 by(cases "x64_decode (unat xpc) ?l_bin",simp_all)
-      done
-    have c3:"?st' = x64_sem (Suc(Suc(Suc(Suc(Suc 0))))) ?l_bin (Next xpc1 xrs1 m1)" 
-      using c3_1 c3_2 d3_0 b3 by (simp add: a7)
-
-    have c4_0:"xpc1 = of_nat (length ?l_bin1)" using d0_1 a7 b3 exec_instr_def by(cases xins1,simp_all)
-    have c4_4:"unat xpc1 = of_nat (0+length ?l_bin1)" using d3_0 of_nat_def c4_0 by simp
-    hence c4_1:"x64_decode (unat xpc1) ?l_bin \<noteq> None" using d4_0 a7 by simp     
-    have c4_2:"?st' = (case x64_decode (unat xpc1) ?l_bin of
-                  None \<Rightarrow> Stuck |
-                 Some (sz, ins) \<Rightarrow>
-              x64_sem (Suc(Suc(Suc(Suc 0)))) ?l_bin (exec_instr ins (of_nat sz) xpc1 xrs1 m1))" 
-      using c3 a3 c0_1 c15 c0 c3_1 apply(cases "Next xpc1 xrs1 m1",simp_all) 
-      apply(cases "prog ! unat pc",simp_all)
-      subgoal for x91 by(cases "x64_decode (unat xpc1) ?l_bin",simp_all)
-      done
-    
-    have c4:"?st' = x64_sem (Suc(Suc(Suc(Suc 0)))) ?l_bin (Next xpc2 xrs2 m2)" 
-      using c4_2 d4_0 c4_4 b4 by simp  
-
-    have c5_1:"xpc2 = xpc1 + of_nat(length ?l_bin2)" using b4 d4_1 d4_2
-      apply(unfold exec_instr_def,simp_all)
-      apply(cases xins2,simp_all)
-      apply(unfold exec_push_def sp_block_def)
-      apply(cases "storev M64 m1 (Vptr 1 (xrs1 (IR SP) - u64_of_memory_chunk M64)) (Vlong (xrs1 (IR RAX)))",simp_all)
-       apply (metis One_nat_def of_nat_1 outcome.simps(3))
-      subgoal for a
-        by (metis d4_2 of_nat_1 outcome.inject)
-      done
-    have c5_2:"xpc2 = of_nat(length ?l_bin1+length ?l_bin2)" using c5_1 c4_0 by simp
-    have "length ?l_bin1+length ?l_bin2 = 4" using f0 f1 by simp 
-    hence c5_3:"unat xpc2 = (0 + length ?l_bin1+length ?l_bin2)" using c5_2 of_nat_def by auto
-    have "\<exists> tempst'. x64_sem (Suc 0) ?l_bin (Next xpc2 xrs2 m2) = tempst' \<and>
-    x64_sem (Suc(Suc(Suc 0))) ?l_bin tempst' = ?st'" using c4 x64_sem_add 
-      using One_nat_def plus_1_eq_Suc by presburger
-    then obtain tempst' where c5_4:"x64_sem (Suc 0) ?l_bin (Next xpc2 xrs2 m2) = tempst' \<and>
-    x64_sem (Suc(Suc(Suc 0))) ?l_bin tempst' = ?st'" by auto
-    have c5_5:"x64_decode (unat xpc2) ?l_bin \<noteq> None" using c5_3 d5_1 by simp
-    have c5_6:"x64_sem (Suc 0) ?l_bin (Next xpc2 xrs2 m2) = tempst'" using c5_4 by auto
-    have c5_7:"x64_decode (0 + length ?l_bin1+length ?l_bin2) ?l_bin = Some (sz3,xins3)" using d5_1 by simp
-    have "tempst' =  (case x64_decode (0 + length ?l_bin1+length ?l_bin2) ?l_bin of
-      None \<Rightarrow> Stuck |
-      Some (sz, ins) \<Rightarrow>
-        x64_sem 0 ?l_bin (exec_instr ins (of_nat sz) xpc2 xrs2 m2))" using c5_3 c5_6
-      by (metis x64_sem.simps(3))
-    hence "tempst' = x64_sem 0 ?l_bin (exec_instr xins3 (of_nat sz3) xpc2 xrs2 m2)" using c5_7 d5_1 c0_1 
-      apply(cases "x64_decode (0 + length ?l_bin1+length ?l_bin2) ?l_bin",simp_all)
-      subgoal for a apply(cases "prog ! unat pc",simp_all) 
-        subgoal for x91 by auto
-        done
-      done
-    hence c5:"tempst' = Next xpc3 xrs3 m3" using b5 by simp
-
-    have c6_0:" x64_sem (Suc(Suc(Suc 0))) ?l_bin tempst' = ?st'" using c5_4 by auto
-    have c6_1:"xpc3 =  xpc2 + of_nat(length ?l_bin3)" using  b5 d6 
-      by(unfold exec_instr_def,simp_all)
-    have c6_2:"xpc3 = of_nat(length ?l_bin1+length ?l_bin2+length ?l_bin3)" using c6_1 c5_2 by auto
-    have "length ?l_bin1+length ?l_bin2+length ?l_bin3=7" using f0 f1 f2 by linarith
-    hence c6_3:"unat xpc3 = (0 + length ?l_bin1+length ?l_bin2+length ?l_bin3)" using c6_2 of_nat_def by auto
-    have "\<exists> tempst'. x64_sem (Suc 0) ?l_bin (Next xpc3 xrs3 m3) = tempst' \<and>
-    x64_sem ((Suc(Suc 0)))?l_bin tempst' = ?st'" using c4 x64_sem_add 
-      using One_nat_def plus_1_eq_Suc c5 c6_0 by presburger
-    then obtain tempst' where c6_4:"x64_sem (Suc 0) ?l_bin (Next xpc3 xrs3 m3) = tempst' \<and>
-    x64_sem ((Suc(Suc 0))) ?l_bin tempst' = ?st'" by auto
-    have c6_5:"x64_decode (unat xpc3) ?l_bin \<noteq> None" using c6_3 d8_1 by simp
-    have c6_6:"x64_sem (Suc 0) ?l_bin (Next xpc3 xrs3 m3) = tempst'" using c6_4 by auto
-    have "tempst' =  (case x64_decode (0 + length ?l_bin1+length ?l_bin2+length ?l_bin3) ?l_bin of
-      None \<Rightarrow> Stuck |
-      Some (sz, ins) \<Rightarrow>
-        x64_sem 0 ?l_bin (exec_instr ins (of_nat sz) xpc3 xrs3 m3))" using c6_3 c6_6
-      by (metis x64_sem.simps(3))
-    hence "tempst' = x64_sem 0 ?l_bin (exec_instr xins4 (of_nat sz4) xpc3 xrs3 m3)" using  d8_1 c6_5
-      by(cases "x64_decode (0 + length ?l_bin1+length ?l_bin2) ?l_bin",simp_all)
-    hence c6:"tempst' = Next xpc4 xrs4 m4" using b6 by simp
-
-    have c7_0:" x64_sem (Suc(Suc 0)) ?l_bin tempst' = ?st'" using c6_4 by auto
-    have c7_1:"xpc4 =  xpc3 + of_nat(length ?l_bin3)" using b6 d9
-      by(unfold exec_instr_def,simp_all)
-    hence c7_2:"xpc4 = of_nat(length ?l_bin1+length ?l_bin2+length ?l_bin3+length ?l_bin4)" using c6_2 by auto
-    have "length ?l_bin1+length ?l_bin2+length ?l_bin3+length ?l_bin4 = 10" using f0 f1 f2 f3 by simp
-    hence c7_3:"unat xpc4 = (0 + length ?l_bin1+length ?l_bin2+length ?l_bin3+length ?l_bin4)" using of_nat_def c7_2 by auto
-    have "\<exists> tempst'. x64_sem (Suc 0) ?l_bin (Next xpc4 xrs4 m4) = tempst' \<and>
-    x64_sem (Suc 0) ?l_bin tempst' = ?st'" using x64_sem_add 
-      using One_nat_def plus_1_eq_Suc c6 c7_0 by presburger
-    then obtain tempst' where c7_4:"x64_sem (Suc 0) ?l_bin (Next xpc4 xrs4 m4) = tempst' \<and>
-    x64_sem (Suc 0) ?l_bin tempst' = ?st'" by auto
-    have c7_5:"x64_decode (unat xpc4) ?l_bin \<noteq> None" using c7_3 d11_1 by simp
-    have c7_6:"x64_sem (Suc 0) ?l_bin (Next xpc4 xrs4 m4) = tempst'" using c7_4 by auto
-    have "tempst' =  (case x64_decode (0 + length ?l_bin1+length ?l_bin2+length ?l_bin3+length ?l_bin4) ?l_bin of
-      None \<Rightarrow> Stuck |
-      Some (sz, ins) \<Rightarrow>
-        x64_sem 0 ?l_bin (exec_instr ins (of_nat sz) xpc4 xrs4 m4))" using c7_3 c7_6
-      by (metis x64_sem.simps(3))
-    hence "tempst' = x64_sem 0 ?l_bin (exec_instr xins5 (of_nat sz5) xpc4 xrs4 m4)" using d11_1
-      by(cases "x64_decode (0 + length ?l_bin1+length ?l_bin2) ?l_bin",simp_all)
-    hence c7:"tempst' = Next xpc5 xrs5 m5" using b7 by simp
-
-    have c8_0:" x64_sem (Suc 0) ?l_bin tempst' = ?st'" using c7_4 by auto
-    have c8_1:"xpc5 =  xpc4 + of_nat(length ?l_bin5)" using b7 d12
-      by(unfold exec_instr_def,simp_all)
-    hence c8_2:"xpc5 = of_nat(length ?l_bin1+length ?l_bin2+length ?l_bin3+length ?l_bin4+length ?l_bin5)" using c7_2 by auto
-    have "length ?l_bin1+length ?l_bin2+length ?l_bin3+length ?l_bin4+length ?l_bin5 = 13" using  f0 f1 f2 f3 f4 by simp
-    hence c8_3:"unat xpc5 = (0 + length ?l_bin1+length ?l_bin2+length ?l_bin3+length ?l_bin4+length ?l_bin5)" using of_nat_def c8_2 by auto
-    have "\<exists> tempst'. x64_sem (Suc 0) ?l_bin (Next xpc5 xrs5 m5) = tempst' \<and>
-    x64_sem 0 ?l_bin tempst' = ?st'" using x64_sem_add 
-      using One_nat_def plus_1_eq_Suc c7 c8_0 by auto
-    then obtain tempst' where c8_4:"x64_sem (Suc 0) ?l_bin (Next xpc5 xrs5 m5) = tempst' \<and>
-    x64_sem 0 ?l_bin tempst' = ?st'" by auto
-    have c8_5:"x64_decode (unat xpc5) ?l_bin \<noteq> None" using c8_3 d14_1 by simp
-    have c8_6:"x64_sem (Suc 0) ?l_bin (Next xpc5 xrs5 m5) = tempst'" using c8_4 by auto
-    have "tempst' =  (case x64_decode (0 + length ?l_bin1+length ?l_bin2+length ?l_bin3+length ?l_bin4+length ?l_bin5) ?l_bin of
-      None \<Rightarrow> Stuck |
-      Some (sz, ins) \<Rightarrow>
-        x64_sem 0 ?l_bin (exec_instr ins (of_nat sz) xpc5 xrs5 m5))" using c8_3 c8_6
-      by (metis x64_sem.simps(3))
-    hence "tempst' = x64_sem 0 ?l_bin (exec_instr xins6 (of_nat sz6) xpc5 xrs5 m5)" using d14_1 
-      by(cases "x64_decode (0 + length ?l_bin1+length ?l_bin2) ?l_bin",simp_all)
-    hence c8:"tempst' = Next xpc6 xrs6 m6" using b8 by simp
-    have cn:"?st' = Next xpc6 xrs6 m6" using c8 c8_4 by simp
-
-  have e1:"(\<forall> r. (rs r) = xrs (IR (bpf_to_x64_reg r)))" using a1 spec match_state_def match_reg_def a4 a3 by simp
-  moreover have e2:"(rs src) = xrs (IR (bpf_to_x64_reg src))" using spec e1 by simp
-  moreover have e2_1:"(rs dst) = xrs (IR (bpf_to_x64_reg dst))" using spec e1 by simp
-  hence e3:"(rs' dst) = xrs6 (IR (bpf_to_x64_reg dst))"            
-    using mulq_subgoal_rr_aux1_2 c2 c0_1 a0 a1 a2 a3 e2 e2_1 c14 c13 by fastforce
-  have " \<forall> r. bpf_to_x64_reg r \<notin> {RDX}\<longrightarrow> xrs6 (IR (bpf_to_x64_reg r)) = xrs (IR (bpf_to_x64_reg r))" 
-    using c13 c14 mulq_subgoal_rr_aux1_4 c2 bpf_to_x64_reg_corr by fastforce
-  hence e4:" \<forall> r\<noteq>dst. xrs6 (IR (bpf_to_x64_reg r)) = xrs (IR (bpf_to_x64_reg r))" 
-    using bpf_to_x64_reg_corr bpf_to_x64_reg_corr2 c2  by (metis singletonD)
-  have e5:"\<forall> r \<noteq> dst. (rs' r) = (rs r)" using mulq_subgoal_rr_aux3 a0 a1 a2 c0_1 by blast
-  have e7:"(\<forall> r \<noteq> dst. (rs' r) = xrs6 (IR (bpf_to_x64_reg r)))" using e1 e4 e5 by presburger
-  have e8:"match_stack xrs6 m6" using mulq_match_stack match_state_def a4 c13 c14 a3 a1 by auto
-  have e9:"match_mem m' m6" using mulq_match_mem match_state_def a4 c13 c14 a3 a1 a0 a1 a2 c0_1 by fastforce
-  have "match_state s' (pc',?st')" using e3 e7 match_state_def e8 e9 match_reg_def cn a2 by fastforce
-  thus ?thesis using c16 by simp
-next
-  case False
-    have c2_1:"(bpf_to_x64_reg dst) = RAX \<or> (bpf_to_x64_reg dst) \<notin> {RAX, RDX}" using c2_0 False by blast
-    thus ?thesis
-    proof (cases "(bpf_to_x64_reg dst) = RAX")
-      case True
-      then show ?thesis sorry
-    next
-      case False
-      have "(bpf_to_x64_reg dst) \<notin> {RAX, RDX}" using c2_1 False by blast
-      then show ?thesis sorry
-    qed   
-  qed 
-    next
-    case True
-    let "?l_bin"= "snd (snd (the (per_jit_ins ?bpf_ins)))"
-    have c1_0:"?l_bin = snd (snd (the (per_jit_jcc cond dst src (scast x))))" using True by auto
-    let "?tcond" = "Cond_e"
-    have c1_1:"cond = Eq" sorry
-    have c1:"?l_bin = (let ins1 = Pcmpq_rr (bpf_to_x64_reg dst) (bpf_to_x64_reg src); ins2 = (Pjcc ?tcond 0) in x64_encode ins1@x64_encode ins2 )" 
-      using c1_1 per_jit_jcc_def c1_0 by simp
-    have c0:"?l_bin = snd (snd (the (per_jit_jcc cond dst src (scast x))))" using b2 True by fastforce
-    have c2:"l = ?l_bin" using a6 c0 a5 aux5 by metis
-    let "?st" = "x64_sem num ?l_bin xst"
-    have "x64_prog!(unat pc) = the (per_jit_ins ?bpf_ins)" using aux5 a5 a6 by blast
-    then have "x64_prog!(unat pc) = the (per_jit_jcc cond dst src (scast x))" using b2 True by simp
-    then have c3_1:"num = 1" using per_jit_jcc_def c1_1 by simp
-
-    let "?l_bin1" = "x64_encode (Pcmpq_rr (bpf_to_x64_reg dst) (bpf_to_x64_reg src))"
-    let "?l_bin2" = "x64_encode (Pjcc ?tcond 0)"
-    have d0:"list_in_list (?l_bin1@?l_bin2) (0::nat) ?l_bin" using list_in_list_prop c1 by metis
-    have d0_0:"list_in_list ?l_bin 0 ?l_bin = list_in_list ?l_bin1 0 ?l_bin \<and> list_in_list ?l_bin2 (0 + length ?l_bin1) ?l_bin" 
-       using list_in_list_concat d0 c1 list_in_list_prop by blast
-    have d0_1:"list_in_list ?l_bin1 0 ?l_bin" using d0 d0_0 by auto
-    have d0_2:"list_in_list ?l_bin2 (0+length ?l_bin1) ?l_bin" using d0 d0_0 by auto
-    hence "\<exists> xins1 sz1. x64_decode 0 ?l_bin = Some (sz1, xins1)" 
-      by (metis c1 d0 list_in_list_concat x64_encode_decode_consistency)
-    then obtain xins1 sz1 where d1:"x64_decode 0 ?l_bin = Some (sz1, xins1)" by auto
-    have d2:"(sz1,xins1) = (3, Pcmpq_rr (bpf_to_x64_reg dst) (bpf_to_x64_reg src))"  using d0_1 x64_encode_decode_consistency d1 by fastforce
-    have c4:"?st = exec_instr xins1 (of_nat sz1) xpc xrs xm" using c3_1 d2 c1 c2 a7 a3 d1 by auto 
-    have c6:"\<exists> xrs' xpc' xm'. ?st = Next xpc' xrs' xm'" using exec_instr_def spec c4 d2 by simp
-    obtain xrs' xpc' xm' where c7:"?st = Next xpc' xrs' xm'" using c6 by auto
-    have "match_state s' (pc',?st)" using jcc_subgoal_rr_generic a0 a1 a2 c7 a4 a3 per_jit_jcc_def b2 c4 True c1_1 d1 by force
-    then show ?thesis using True c0_0 False c2 by simp
-    qed
-  qed
-qed
-*)
-
-
-
-
-
-
-lemma demo1: 
-  assumes a0:"s' = sbpf_step prog s" and
-  a1:"s = (SBPF_OK pc rs m)" and
-  a2:"s' = (SBPF_OK pc' rs' m')" and
-  a3:"xst = (Next xpc xrs xm)" and
-  a4:"match_state s (pc,xst)" and
-  a5:"jitper prog = Some x64_prog" and                      
-  a6:"prog \<noteq> [] \<and> unat pc < length prog \<and> unat pc \<ge> 0" and
-  a7:"xpc = 0"
+  a6:"prog \<noteq> [] \<and> unat pc < length prog \<and> unat pc \<ge> 0" 
 shows "\<exists> xst'. x64_sem1 1 x64_prog (pc,xst) = (pc',xst') \<and> 
   match_state s' (pc',xst')"
 (* \<and> snd xst' = unat (pc+1)*)
@@ -438,7 +45,7 @@ proof-
       then show ?thesis
       proof(cases "(bpf_to_x64_reg dst) = RDX")
         case True   
-          then show ?thesis using mulq_one_step a0 a1 a2 a3 a4 a5 a6 a7 True c1 c0 by blast
+          then show ?thesis using mulq_one_step a0 a1 a2 a3 a4 a5 a6 True c1 c0 by blast
         next
         case False
           have c2:"(bpf_to_x64_reg dst) = RAX \<or> (bpf_to_x64_reg dst) \<notin> {RAX, RDX}" using c1 False by simp
@@ -458,70 +65,37 @@ proof-
       thus ?thesis 
       proof(cases "(?bpf_ins = BPF_JUMP cond dst (SOReg src) x)")
         case True
-          then show ?thesis using True False a0 a1 a2 a3 a4 a5 a6 a7 jump_one_step by blast
+          then show ?thesis using True False a0 a1 a2 a3 a4 a5 a6 jump_one_step by blast
         next
         case False
           have c5:"?bpf_ins = BPF_ALU64 BPF_ADD dst (SOReg src)" using False c4 by simp
-          then show ?thesis using False a0 a1 a2 a3 a4 a5 a6 a7 addq_one_step c5 by blast
+          then show ?thesis using False a0 a1 a2 a3 a4 a5 a6 addq_one_step c5 by blast
       qed
     qed
   qed
 
-(*lemma x64_sem1_induct_aux1:
-  "x64_sem1 (Suc n) x64_prog (pc, Next xpc xrs m) = xst'\<Longrightarrow> 
-  x64_prog!(unat pc) = (num,off,l) \<Longrightarrow>
-  x64_sem num l (Next 0 xrs m) = xst1 \<Longrightarrow> 
-  xst1 = Next xpc1 xrs1 m1 \<Longrightarrow>
-  x64_sem1 n x64_prog (off+pc,xst1) = xst' \<or> x64_sem1 n x64_prog (pc+1,xst1) = xst'"
-  sorry*)
- (*apply(induct n arbitrary: x64_prog pc xpc xrs m xst' num off l xst1 off')
-   apply simp
-  have 
-  by simp*)
-
-
 lemma x64_sem1_induct_aux1:
-  "s =  SBPF_OK pc rs m \<Longrightarrow>
-  s' = sbpf_step prog s \<Longrightarrow> 
-  s' = SBPF_OK pc' rs' m' \<Longrightarrow> 
-  x64_sem1 (Suc n) x64_prog (pc, Next xpc xrs xm) = xst'\<Longrightarrow> 
-  x64_sem1 1 x64_prog (pc,xst) = (pc1,xst1) \<Longrightarrow> 
-  xst1 = Next xpc1 xrs1 m1 \<Longrightarrow>
-  x64_sem1 n x64_prog (pc',xst1) = xst'"
-  sorry
+ "x64_sem1 (m+n) x64_prog xst = xst'\<Longrightarrow> 
+  \<exists> xst1. x64_sem1 m x64_prog xst = xst1 \<and>
+  x64_sem1 n x64_prog xst1 = xst'"
+ apply(induct m arbitrary: n x64_prog xst xst' )
+   apply auto[1]
+  subgoal for m n x64_prog xst xst'
+    apply (simp add: Let_def)
+    apply(cases xst;simp)
+    done
+  done
 
-lemma x64_sem1_induct_aux2:"x64_sem1 n x64_prog (pc,Next xpc xrs xm) = x64_sem1 n x64_prog (pc,Next 0 xrs xm)"
-  sorry
-(*proof(cases n)
-  case 0
-  then show ?thesis by simp
-next
-  case (Suc n)
-  thus ?thesis using Suc
-    apply(cases "x64_prog ! unat pc",simp_all)
-    subgoal for a b c   apply(cases "Next xpc xrs xm",simp_all)
-      subgoal for x11 
-    apply(split if_splits)
-
-    by fastforce
-qed*)
- 
 lemma x64_sem1_induct_aux3:
-  "s =  SBPF_OK pc rs m \<Longrightarrow>
-  s' = sbpf_step prog s \<Longrightarrow> 
-  s' = SBPF_OK pc' rs' m' \<Longrightarrow> 
-  xst = (Next xpc xrs xm) \<Longrightarrow>
-  x64_sem1 (Suc n) x64_prog (pc,xst) = xst' \<Longrightarrow> 
+  "x64_sem1 (Suc n) x64_prog xst = xst' \<Longrightarrow> 
   x64_prog!(unat pc) = (num,off,l) \<Longrightarrow>
-  x64_sem1 1 x64_prog (pc,xst) = (pc1,xst1)  \<Longrightarrow> 
-  xst1 = Next xpc1 xrs1 m1 \<Longrightarrow>
-  x64_sem1 n x64_prog (pc', Next 0 xrs1 m1) = xst'"
-  using x64_sem1_induct_aux1 x64_sem1_induct_aux2 by metis
+  x64_sem1 1 x64_prog xst = xst1 \<Longrightarrow> 
+  x64_sem1 n x64_prog xst1 = xst'"  
+using x64_sem1_induct_aux1
+  by (metis plus_1_eq_Suc)
 
 
-
-
-lemma demo2_aux:
+lemma n_steps_equiv_proof_aux:
   "\<lbrakk> sbpf_sem n prog s = s';
    s = (SBPF_OK pc rs m);
    s' = (SBPF_OK pc' rs' m');
@@ -529,11 +103,10 @@ lemma demo2_aux:
    match_state s (pc,xst);
    jitper prog = Some x64_prog;
    prog \<noteq> [];
-   xpc = 0;
    x64_sem1 n x64_prog (pc,xst) = xst' \<rbrakk> \<Longrightarrow>
    match_state s' xst'"
 (* \<exists> xst'. x64_sem1 n pc x64_prog xst = xst' \<and> match_state s' xst'"*)
-proof (induction n arbitrary: prog s s' pc rs m pc' rs' m' xst' xst xpc xrs xm x64_prog idx xst')
+proof (induction n arbitrary: prog s s' pc rs m pc' rs' m' xst' xst xpc xrs xm x64_prog xst')
   case 0
   then show ?case
     by simp
@@ -547,7 +120,6 @@ next
        assm5:"match_state s (pc,xst)" and
        assm6:"jitper prog = Some x64_prog" and
        assm7:"prog \<noteq> [] " and
-       assm8:"xpc = 0" and
        assm9:"x64_sem1 (Suc n) x64_prog (pc,xst) = xst'"
   then obtain s1 where s1_eq: "s1 = sbpf_step prog s" by simp
   have n_step_def:"sbpf_sem n prog s1 = s'" using s1_eq assm1 sbpf_sem_induct
@@ -564,16 +136,12 @@ next
   have a7:"l = (snd (snd ((x64_prog!(unat pc)))))" using a6 by simp
 
   have "\<exists> xst1. x64_sem1 1 x64_prog (pc,xst) = (pc1,xst1) \<and> match_state s1 (pc1,xst1)"
-    using s1_eq assm2 a2 assm4 assm5 assm6 assm7 assm8 demo1 a6 a7 a0 by blast
+    using s1_eq assm2 a2 assm4 assm5 assm6 assm7 one_step_equiv_proof a6 a7 a0 by blast
   then obtain xst1 where a4:"x64_sem1 1 x64_prog (pc,xst) = (pc1,xst1) \<and> match_state s1 (pc1,xst1)" by auto
-  (*have "\<exists> xst1. x64_sem num l (Next xpc xrs xm) = xst1 \<and> match_state s1 (pc1,xst1)"
-    using s1_eq assm2 a2 assm4 assm5 assm6 assm7 assm8 assm8 demo1 a6 a7 by (metis (mono_tags, lifting) calculation)
-  then obtain xst1 where a4:"x64_sem ?num (snd (snd ((x64_prog!(unat pc)))))(Next 0 xrs xm) = xst1 \<and> match_state s1 (pc1,xst1)" using assm8 by auto*)
   hence a4_1:"x64_sem1 1 x64_prog (pc,xst) = (pc1,xst1)" by auto
   have an:"\<exists> xpc1 xrs1 xm1. xst1 = Next xpc1 xrs1 xm1" using a4 by (metis match_s_not_stuck outcome.exhaust)
   then obtain xpc1 xrs1 xm1 where a10:"xst1 = Next xpc1 xrs1 xm1" by auto
-  let "?xst1" = "Next 0 xrs1 xm1"
-  have a5:"match_state s1 (pc1,?xst1)" using an match_state_def
+  have a5:"match_state s1 (pc1,xst1)" using an match_state_def
     using a10 a2 a4 by fastforce
   have    "sbpf_sem n prog s = s' \<Longrightarrow>
            s = SBPF_OK pc rs m \<Longrightarrow>
@@ -582,42 +150,21 @@ next
            match_state s (pc, xst) \<Longrightarrow>
            jitper prog = Some x64_prog \<Longrightarrow> 
            prog \<noteq> [] \<Longrightarrow> 
-           xpc = (0::64 word) \<Longrightarrow> 
            x64_sem1 n x64_prog (pc, xst) = xst' \<Longrightarrow> 
            match_state s' xst'" using Suc by blast
-  have "x64_sem1 n x64_prog (pc1, ?xst1) = xst'" 
-    using x64_sem1_induct_aux3 a2 assm2 s1_eq assm4 assm9 a6 a4 a10 
-    by (metis (full_types) x64_sem1_induct_aux3)
-  hence "match_state s' xst'"
-    using n_step_def a2 assm3 a10 a5 assm6 assm7 assm8 Suc by blast
-  hence an:"match_state s' xst'" by blast
+  
+  have "\<exists> xst''. x64_sem1 n x64_prog (pc1, xst1) = xst''" by blast
+  then obtain xst'' where b0:"x64_sem1 n x64_prog (pc1, xst1) = xst''" by auto
+  hence b1:"xst' = xst''" 
+    using x64_sem1_induct_aux1 a2 assm2 s1_eq assm4 assm9 a6 a4 a10 by (metis plus_1_eq_Suc)
+  hence "match_state s' xst''"
+    using n_step_def a2 assm3 a10 a5 assm6 assm7 Suc b0 by simp
+  hence an:"match_state s' xst'" using b1 by simp
   then show ?case using an by auto
 qed
 
 
-(* 
-  "s =  SBPF_OK pc rs m \<Longrightarrow>
-  s' = sbpf_step prog s \<Longrightarrow> 
-  s' = SBPF_OK pc' rs' m' \<Longrightarrow> 
-  x64_sem1 (Suc n) x64_prog (pc, Next xpc xrs m) = xst'\<Longrightarrow> 
-  x64_prog!(unat pc) = (num,off,l) \<Longrightarrow>
-  x64_sem num l (Next 0 xrs m) = xst1 \<Longrightarrow> 
-  xst1 = Next xpc1 xrs1 m1 \<Longrightarrow>
-  x64_sem1 n x64_prog (off+pc,xst1) = xst' \<or> x64_sem1 n x64_prog (pc+1,xst1) = xst'"
-
-"jitper prog = Some x64_prog \<Longrightarrow>
-  prog \<noteq> [] \<and> unat pc \<ge> 0 \<and> unat pc < length prog \<Longrightarrow>
-  prog!(unat pc) = bin \<Longrightarrow>
-  bin = BPF_JUMP cond dst src d \<Longrightarrow>
-  s =  SBPF_OK pc rs m \<Longrightarrow>
-  s' = sbpf_step prog s \<Longrightarrow> 
-  s' = SBPF_OK pc' rs' m' \<Longrightarrow> 
-  (num,off,l) = x64_prog!(unat pc) \<Longrightarrow>
-  pc' = pc + off"*)
-
-
-
-lemma demo2:
+lemma n_steps_equiv_proof:
   "\<lbrakk> sbpf_sem n prog s = s';
    s = (SBPF_OK pc rs m);
    s' = (SBPF_OK pc' rs' m');
@@ -628,8 +175,8 @@ lemma demo2:
    xpc = 0 \<rbrakk> \<Longrightarrow>
    \<exists> xst'.  x64_sem1 n x64_prog (pc,xst) = (pc',xst') \<and>
    match_state s' (pc',xst')"
-  using demo2_aux
-  sorry
+  using n_steps_equiv_proof_aux sorry
+  
 
                                  
 end
