theory/JITPer_exit.thy
@@ -20,16 +20,16 @@ proof-
   have b0:"st' = SBPF_Success (rs BR0)" using a0 a4 a7 a8 by simp
   have b1:"xins = Pret" using x64_encode_decode_consistency per_jit_exit_def a0 a1 a3 list_in_list_prop
     by (smt (verit, ccfv_SIG) map_option_eq_Some option.inject prod.inject)
-  moreover have b2:"(\<forall> r. (rs r) = reg (bpf_to_x64_reg r))" using a6 spec match_state_def match_reg_def by simp
-  moreover have b3:"(rs BR0) = reg (bpf_to_x64_reg BR0)" using a6 spec b2 by simp
+  moreover have b2:"(\<forall> r. (rs  r) = reg (IR (bpf_to_x64_reg r)))" using a6 spec match_state_def match_reg_def by simp
+  moreover have b3:"(rs BR0) = reg (IR (bpf_to_x64_reg BR0))" using a6 spec b2 by simp
   (*have b4:"Mem.loadv M64 m ((reg SP) + (u64_of_memory_chunk M64)) \<noteq> None" using match_state_def a6 match_stack_def by auto
   hence "\<exists> x. Mem.loadv M64 m ((reg SP) + (u64_of_memory_chunk M64)) = x \<and> x\<noteq> None" by simp
   hence "\<exists> v. Mem.loadv M64 m ((reg SP) + (u64_of_memory_chunk M64)) = Some v" by simp*)
-  hence b5_1:"\<exists> v. Mem.loadv M64 m (Vlong ((reg SP) + (u64_of_memory_chunk M64))) = Some (Vlong v)" using match_state_def a6 match_stack_def by simp
-  obtain v where b5_2:"Mem.loadv M64 m (Vlong ((reg SP) + (u64_of_memory_chunk M64))) = Some (Vlong v)" using b5_1 by blast
-  let "?reg'" = "(reg#SP <- ((reg SP) + (u64_of_memory_chunk M64)))"
+  hence b5_1:"\<exists> v. Mem.loadv M64 m (Vlong ((reg (IR SP)) + (u64_of_memory_chunk M64))) = Some (Vlong v)" using match_state_def a6 match_stack_def by simp
+  obtain v where b5_2:"Mem.loadv M64 m (Vlong ((reg (IR SP)) + (u64_of_memory_chunk M64))) = Some (Vlong v)" using b5_1 by blast    
+  let "?reg'" = "(reg#(IR SP) <- ((reg (IR SP)) + (u64_of_memory_chunk M64)))"
   have b5_3:"xst' = Next v ?reg' m" using exec_instr_def exec_ret_def a5 b1 b5_2 by simp
-  hence b5:"?reg' (bpf_to_x64_reg BR0) = reg (bpf_to_x64_reg BR0)" by (simp add: bpf_to_x64_reg_def)
+  hence b5:"?reg' (IR (bpf_to_x64_reg BR0)) = reg (IR (bpf_to_x64_reg BR0))" by (simp add: bpf_to_x64_reg_def)
   thus ?thesis using exec_instr_def b3 b1 b0 a5 using b5_2 exec_ret_def match_state_def by force
 qed
 
