theory/JITPer_jump.thy
@@ -59,28 +59,43 @@ lemma jump_one_step:
   a4:"match_state s (pc,xst)" and
   a5:"jitper prog = Some x64_prog" and                      
   a6:"prog \<noteq> [] \<and> unat pc < length prog \<and> unat pc \<ge> 0" and
-  a7:"xpc = 0" and
   a8:"prog!(unat pc) = BPF_JUMP cond dst (SOReg src) x"
 shows "\<exists> xst'. x64_sem1 1 x64_prog (pc,xst) = (pc',xst') \<and> 
   match_state s' (pc',xst')"
 proof-
     let "?bpf_ins" = "prog!(unat pc)"
     let "?l_bin"= "snd (snd (the (per_jit_ins ?bpf_ins)))"
-    have c1_0:"?l_bin = snd (snd (the (per_jit_jcc cond dst src (scast x))))" using a8 by auto
+    have c1_0:"?l_bin = snd (snd (the (per_jit_jcc cond dst src (scast x))))" using a8 per_jit_ins_def by auto
     let "?tcond" = "Cond_e"
     have c1_1:"cond = Eq" sorry
     have c1:"?l_bin = (let ins1 = Pcmpq_rr (bpf_to_x64_reg dst) (bpf_to_x64_reg src); ins2 = (Pjcc ?tcond 0) in x64_encode ins1@x64_encode ins2 )" 
       using c1_1 per_jit_jcc_def c1_0 by simp
-    have c0:"?l_bin = snd (snd (the (per_jit_jcc cond dst src (scast x))))" using a8 by fastforce
+    have c0:"?l_bin = snd (snd (the (per_jit_jcc cond dst src (scast x))))" using a8 per_jit_ins_def by fastforce
 
     have "\<exists> num off l. x64_prog!(unat pc) = (num,off,l)" by (metis split_pairs)
     then obtain num off l where c_aux:"x64_prog!(unat pc) = (num,off,l)" by auto
 
     have c2:"l = ?l_bin" using a6 c0 a5 aux5 c_aux by fastforce
-    let "?st" = "x64_sem num ?l_bin xst"
-    have "x64_prog!(unat pc) = the (per_jit_ins ?bpf_ins)" using aux5 a5 a6 by blast
-    then have c3:"x64_prog!(unat pc) = the (per_jit_jcc cond dst src (scast x))" using a8 by simp
+      
+    let "?one_step" = "x64_sem1 1 x64_prog (pc,xst)"
+    let "?st" = "snd ?one_step"
+    have c2_1:"?st = snd (one_step x64_prog (pc,xst))" 
+      by (metis One_nat_def prod.collapse x64_sem1.simps(1) x64_sem1.simps(2))
+
+    have c3_0:"x64_prog!(unat pc) = the (per_jit_ins ?bpf_ins)" using aux5 a5 a6 by blast
+    then have c3:"x64_prog!(unat pc) = the (per_jit_jcc cond dst src (scast x))" using a8 per_jit_ins_def by simp
+    have c3_0:"per_jit_jcc cond dst src (scast x) = Some (num,off,l)" using c_aux c3 c1_1 per_jit_jcc_def by auto
     then have c3_1:"num = 1" using per_jit_jcc_def c1_1 c_aux by simp
+
+    have e3_0:"off = scast x + 1" using c_aux per_jit_jcc_def c3 c1_1 by simp
+    have e3:"off\<noteq>0" sorry
+    have "?st = snd (let xst_temp = Next 0 xrs xm; xst' = x64_sem num l xst_temp in
+        case xst' of Next xpc' rs' m' \<Rightarrow>
+          if rs' (CR ZF) = 1 then (off+pc, xst')
+          else (pc+1, xst') |
+         Stuck \<Rightarrow> (pc, Stuck))" using c2_1 e3 a3 one_step_def c_aux by simp
+    hence e3_1:"?st = x64_sem num ?l_bin (Next 0 xrs xm)" using c2_1 c_aux one_step_def e3 a3
+      by (smt (verit, ccfv_threshold) c2 outcome.exhaust outcome.simps(4) outcome.simps(5) snd_conv) 
 
     let "?l_bin1" = "x64_encode (Pcmpq_rr (bpf_to_x64_reg dst) (bpf_to_x64_reg src))"
     let "?l_bin2" = "x64_encode (Pjcc ?tcond 0)"
@@ -93,13 +108,11 @@ proof-
       by (metis c1 d0 list_in_list_concat x64_encode_decode_consistency)
     then obtain xins1 sz1 where d1:"x64_decode 0 ?l_bin = Some (sz1, xins1)" by auto
     have d2:"(sz1,xins1) = (3, Pcmpq_rr (bpf_to_x64_reg dst) (bpf_to_x64_reg src))"  using d0_1 x64_encode_decode_consistency d1 by fastforce
-    have c4:"?st = exec_instr xins1 (of_nat sz1) xpc xrs xm" using c3_1 d2 c1 c2 a7 a3 d1 by auto 
+    have c4:"?st = exec_instr xins1 (of_nat sz1) 0 xrs xm" using c3_1 d2 c1 c2 a3 d1 e3_1 by auto 
     have c6:"\<exists> xrs' xpc' xm'. ?st = Next xpc' xrs' xm'" using exec_instr_def spec c4 d2 by simp
     obtain xrs' xpc' xm' where c7:"?st = Next xpc' xrs' xm'" using c6 by auto
-    have cn:"x64_sem num l xst = ?st \<and> match_state s' (pc',?st)" 
-      using jcc_subgoal_rr_generic a0 a1 a2 c7 a4 a3 per_jit_jcc_def a8 c4 c1_1 d1 c2 c7 by force
-    
-    have "exec_instr xins1 (of_nat sz1) xpc xrs xm = Next (xpc+(of_nat sz1))(compare_longs (xrs (IR (bpf_to_x64_reg src))) (xrs (IR (bpf_to_x64_reg dst))) xrs) xm"
+  
+    have e0_1:"exec_instr xins1 (of_nat sz1) 0 xrs xm = Next (0+(of_nat sz1))(compare_longs (xrs (IR (bpf_to_x64_reg src))) (xrs (IR (bpf_to_x64_reg dst))) xrs) xm"
       using  exec_instr_def d2 a3 by simp
      
     hence e0:"let x = xrs (IR (bpf_to_x64_reg src)); y = xrs (IR (bpf_to_x64_reg dst)) in
@@ -109,12 +122,17 @@ proof-
                             #(CR OF) <- (sub_overflowi64 x y 0))"
       using c7 c4 d2 c4 a3 exec_instr_def of_optbool_def a8
       by (simp add: compare_longs_def)    
-    hence e1:"xrs (IR (bpf_to_x64_reg dst)) = xrs (IR (bpf_to_x64_reg src)) \<longrightarrow>xrs' (CR ZF) = 1" by (smt (verit, del_insts) crbit.distinct(1) crbit.distinct(5) crbit.distinct(7)  fun_upd_apply preg.inject(2) x64Semantics.of_optbool_def)
-    have e2:"xrs (IR (bpf_to_x64_reg dst)) \<noteq> xrs (IR (bpf_to_x64_reg src)) \<longrightarrow>xrs' (CR ZF) = 0" by (smt (verit, del_insts) crbit.distinct(1) crbit.distinct(5) crbit.distinct(7) e0 fun_upd_apply preg.inject(2) x64Semantics.of_optbool_def)
-    have e3_0:"off = scast x + 1" using c_aux per_jit_jcc_def c3 c1_1 by simp
-    have e3:"off\<noteq>0" sorry
-    have "x64_sem1 1 x64_prog (pc,xst) = (pc', Next 0 xrs' xm')"
-      using a8 e1 e2 cn a0 a1 a2 a3 a4 a5 a6 a7 x64_sem1_pc_aux1 c_aux match_state_eqiv e3 c7 x64_sem1_pc_aux2 by auto
+    hence e1:"xrs (IR (bpf_to_x64_reg dst)) = xrs (IR (bpf_to_x64_reg src)) \<longrightarrow>xrs' (CR ZF) = 1" 
+      by (smt (verit, del_insts) crbit.distinct(1) crbit.distinct(5) crbit.distinct(7)  fun_upd_apply preg.inject(2) x64Semantics.of_optbool_def)
+    have e2:"xrs (IR (bpf_to_x64_reg dst)) \<noteq> xrs (IR (bpf_to_x64_reg src)) \<longrightarrow>xrs' (CR ZF) = 0" 
+      by (smt (verit, del_insts) crbit.distinct(1) crbit.distinct(5) crbit.distinct(7) e0 fun_upd_apply preg.inject(2) x64Semantics.of_optbool_def)
+
+    have cn_1:"match_state s (pc,(Next 0 xrs xm))" using a4 match_state_eqiv a3 by blast  
+    have cn:"x64_sem num l (Next 0 xrs xm) = ?st \<and> match_state s' (pc',?st)"
+      using jcc_subgoal_rr_generic a0 a1 a2 c7 per_jit_jcc_def a8  c1_1 d1 c2 e3_1 c3_0 c3 c_aux e0_1 c4 cn_1 by metis
+      
+    have "x64_sem1 1 x64_prog (pc,xst) = (pc', Next xpc' xrs' xm')"
+      using a8 e1 e2 cn a0 a1 a2 a3 a4 a5 a6 x64_sem1_pc_aux1 c_aux match_state_eqiv e3 c7 x64_sem1_pc_aux2 by auto
     then show ?thesis using a8 c2 match_state_eqiv c7 cn by fastforce
     qed
 
